lib/loops: Simplify loop lemma
Separate proof into two steps:

1. Prove a lemma that assumes that the user-supplied loop body is responsible
   for incrementing the loop counter.

2. Prove a lemma that automatically implement the counter, with a simpler
   post-condition for the body: instead of forcing the invariant to hold over
   the final state (after incrementing the counter), require that the invariant
   should not use the counter for anything except tracking the counter variable
   in the ‘locals’ map.

The new shape of the body post-condition requires an additional property for the
loop invariant, but it should be straightforward to prove.

src/Rupicola/Lib/Loops.v
@@ -3,18 +3,27 @@ Require Import Rupicola.Lib.Api.
 
 Module Type ExitToken_sig.
   Axiom t : Set.
-  Axiom new : bool -> t.
+  Axiom new : t.
   Axiom get : t -> bool.
-  Axiom set : t -> t.
+  Axiom break : t -> t.
+  Axiom continue : t -> t.
 End ExitToken_sig.
 
 Module ExitToken <: ExitToken_sig.
+  (* TODO figure out a representation that lets us store ExitToken.t in the same
+     variable as the loop counter *)
   Definition t := bool.
-  Definition new (b: bool) : t := b.
+  Definition new : t := false.
   Definition get (tok: t) : bool := tok.
-  Definition set (tok: t) : t := true.
-  Definition branch {A} (tok: t) (set unset: A) :=
-    if tok then set else unset.
+  Definition break (tok: t) : t := true.
+  Definition continue (tok: t) : t := false.
+  Definition branch {T} (tok: t) (break continue: T) :=
+    if tok then break else continue.
+
+  Lemma map_branch {T1 T2} (f: T1 -> T2) tok break continue:
+    f (branch tok break continue) =
+    branch tok (f break) (f continue).
+  Proof. destruct tok; reflexivity. Qed.
 End ExitToken.
 
 Open Scope Z_scope.
@@ -399,7 +408,7 @@ Proof. lia. Qed.
 (* Lemma ranged_for_break_continue_eqn {A} from to step body a0 *)
 (*       (H: forall idx, _) H': *)
 (*   @ranged_for_break A from (to + step) step body a0  = *)
-(*   snd (body (ExitToken.new false) to *)
+(*   snd (body ExitToken.new to *)
 (*             (ranged_for_break from to step *)
 (*                         (fun tok idx acc pr => *)
 (*                            body tok idx acc (H idx pr)) *)
@@ -427,19 +436,27 @@ Section WithTok.
       ranged_for_break
         from to
         (fun idx acc pr =>
-           body (ExitToken.new false) idx (snd acc) pr)
+           body ExitToken.new idx (snd acc) pr)
         (fun tok_acc => ExitToken.get (fst tok_acc))
-        (ExitToken.new false, a0).
+        (ExitToken.new, a0).
 
     Definition ranged_for :=
       snd ranged_for'.
+
+    Lemma ranged_for_exit :
+      from >= to ->
+      ranged_for = a0.
+    Proof.
+      unfold ranged_for, ranged_for'; intros.
+      rewrite ranged_for_break_exit; eauto.
+    Qed.
 
     Definition ranged_for_nobreak :=
       snd (ranged_for_all
              from to
              (fun idx acc pr =>
-                body (ExitToken.new false) idx (snd acc) pr)
-             (ExitToken.new false, a0)).
+                body ExitToken.new idx (snd acc) pr)
+             (ExitToken.new, a0)).
   End Def.
 
   Lemma ranged_for'_Proper :
@@ -460,7 +477,7 @@ Section WithTok.
     ranged_for' from (to + 1) body a0 =
     let butlast := ranged_for' from to wbody a0 in
     if fst butlast then butlast
-    else body (ExitToken.new false) to (snd butlast) H.
+    else body ExitToken.new to (snd butlast) H.
   Proof.
     unfold ranged_for'.
     erewrite ranged_for_break_unfold_r.
@@ -472,7 +489,7 @@ Section WithTok.
     (forall t, body_pointwise (body t) (body' t)) ->
     fst (ranged_for' from to body a0) = false ->
     ranged_for' from (to + 1) body' a0 =
-    body' (ExitToken.new false) to (snd (ranged_for' from to body a0)) H.
+    body' ExitToken.new to (snd (ranged_for' from to body a0)) H.
   Proof.
     unfold ranged_for'; intros Hb Hc.
     erewrite ranged_for_break_unfold_r_nstop; eauto; cbv beta; eauto.
@@ -594,19 +611,53 @@ Section with_parameters.
 
     Context (signed: bool).
 
-    Lemma compile_ranged_for A {tr mem locals functions}
+    Lemma lts_of_Z x y:
+      - 2 ^ (Semantics.width - 1) <= x < 2 ^ (Semantics.width - 1) ->
+      - 2 ^ (Semantics.width - 1) <= y < 2 ^ (Semantics.width - 1) ->
+      word.lts (word.of_Z x) (word.of_Z y) = (x <? y).
+    Proof.
+      intros; rewrite word.signed_lts, !word.signed_of_Z, !word.swrap_inrange; eauto.
+    Qed.
+
+    Lemma ltu_of_Z x y:
+      0 <= x < 2 ^ Semantics.width ->
+      0 <= y < 2 ^ Semantics.width ->
+      word.ltu (word.of_Z x) (word.of_Z y) = (x <? y).
+    Proof.
+      intros; rewrite word.unsigned_ltu, !word.unsigned_of_Z, !word.wrap_small; eauto.
+    Qed.
+
+    Lemma getmany0 l t vt vx vy x y:
+      map.getmany_of_list l (vx :: vy :: vt) = Some (x :: y :: t) ->
+      map.get l vx = Some x.
+    Proof.
+      intros; eapply (map.getmany_of_list_get _ 0); eauto || reflexivity.
+    Qed.
+
+    Lemma getmany1 l t vt vx vy x y:
+      map.getmany_of_list l (vx :: vy :: vt) = Some (x :: y :: t) ->
+      map.get l vy = Some y.
+    Proof.
+      intros; eapply (map.getmany_of_list_get _ 1); eauto || reflexivity.
+    Qed.
+
+    Notation in_signed_bounds x :=
+      (- 2 ^ (Semantics.width - 1) <= x < 2 ^ (Semantics.width - 1)).
+
+    Notation in_unsigned_bounds x :=
+      (0 <= x < 2 ^ Semantics.width).
+
+    Lemma _compile_ranged_for A {tr mem locals functions}
           (from to: Z) body (a0: A) :
       let v := ranged_for from to body a0 in
       forall {P} {pred: P v -> predicate}
-        (loop_pred: Z -> A -> predicate)
+        (loop_pred: forall (idx: Z) (a: A), predicate)
         {k: nlet_eq_k P v} {k_impl} {body_impl}
         (from_var to_var: string) vars,
 
         let lp from tok_acc tr mem locals :=
-            let frm := ExitToken.branch (fst tok_acc) (to - 1) from in
-            map.get locals from_var = Some (word.of_Z frm) /\
-            loop_pred (frm + 1) (snd tok_acc) tr mem
-                      (map.put locals from_var (word.of_Z (frm + 1))) in
+            let from := ExitToken.branch (fst tok_acc) to (from + 1) in
+            loop_pred from (snd tok_acc) tr mem locals in
 
         (forall from a0 tr mem locals,
             loop_pred from a0 tr mem locals ->
@@ -614,11 +665,9 @@ Section with_parameters.
             Some [word.of_Z from; word.of_Z to]) ->
 
         loop_pred from a0 tr mem locals ->
-        from <= to ->
-        (if signed then
-           - 2 ^ (Semantics.width - 1) <=  from /\ to < 2 ^ (Semantics.width - 1)
-         else
-           0 <= from /\ to < 2 ^ Semantics.width) ->
+
+        (if signed then in_signed_bounds from /\ in_signed_bounds to
+         else in_unsigned_bounds from /\ in_unsigned_bounds to) ->
 
         ((* loop body *)
           let lp := lp in
@@ -626,19 +675,20 @@ Section with_parameters.
             (Hl: from - 1 < from')
             (Hr: from' < to)
             (Hr': from' <= to),
-            let tok := ExitToken.new false in
             let a := ranged_for' from from' (wbody body pr Hr') a0 in
-            ExitToken.get (fst a) = false ->
-            loop_pred from' (snd a) tr mem locals ->
+            let prev_tok := fst a in
+            let acc := snd a in  (* FIXME use primitive projections? *)
+            ExitToken.get prev_tok = false ->
+            loop_pred from' acc tr mem locals ->
             (<{ Trace := tr;
                 Memory := mem;
                 Locals := locals;
                 Functions := functions }>
              body_impl
-             <{ lp from' (body tok from' (snd a) (conj Hl Hr)) }>)) ->
+             <{ lp from' (body ExitToken.new from' acc (conj Hl Hr)) }>)) ->
         (let v := v in
-         forall tr mem locals,
-           loop_pred to v tr mem locals ->
+         forall from' tr mem locals,
+           loop_pred from' v tr mem locals ->
            (<{ Trace := tr;
                Memory := mem;
                Locals := locals;
@@ -654,17 +704,28 @@ Section with_parameters.
              (expr.op (if signed then bopname.lts else bopname.ltu)
                       (expr.var from_var)
                       (expr.var to_var))
-             (cmd.seq
-                body_impl
-                (cmd.set from_var
-                         (expr.op bopname.add
-                                  (expr.var from_var)
-                                  (expr.literal 1)))))
+             body_impl)
           k_impl
         <{ pred (nlet_eq vars v k) }>.
     Proof.
-      intros * Hlocals Hinit Hfromto Hbounds Hbody Hk.
+      intros * Hlocals Hinit Hbounds Hbody Hk.
       repeat straightline'.
+
+      destruct (Z_gt_le_dec from to).
+      { (* Loop won't run at all *)
+        eexists nat, lt, (fun n tr mem locals => loop_pred from a0 tr mem locals);
+          repeat apply conj; eauto using lt_wf, 0%nat.
+
+        intros.
+        exists (word.of_Z 0); repeat apply conj.
+        - eexists; split; eauto using getmany0.
+          eexists; split; eauto using getmany1.
+          pose proof Zlt_cases from to.
+          destruct signed; simpl; rewrite ?lts_of_Z, ?ltu_of_Z by tauto;
+            destruct (from <? to); reflexivity || lia.
+        - rewrite word.unsigned_of_Z_0; intros; exfalso; lia.
+        - intros. apply (Hk from).
+          subst v. rewrite ranged_for_exit; eauto || lia. }
 
       pose (inv := (fun n tr mem locals =>
                      exists from' (Hr: from' <= to),
@@ -692,39 +753,30 @@ Section with_parameters.
         destruct Hinv as (from' & Hl & Hr & -> & Hcontinue & Hpred).
         eexists ?[b]; split; [|split].
         { (* loop test can be eval'd *)
-          eexists; split;
-            [ eapply (map.getmany_of_list_get _ 0); eauto || reflexivity | ].
-          eexists; split;
-            [ eapply (map.getmany_of_list_get _ 1); eauto || reflexivity | ].
-          [b]: destruct signed.
-          destruct signed; simpl.
-          - rewrite word.signed_lts, !word.signed_of_Z, !word.swrap_inrange by lia;
-              reflexivity.
-          - rewrite word.unsigned_ltu, !word.unsigned_of_Z, !word.wrap_small by lia;
-              reflexivity. }
-        all: intros Hnz; destruct (from' <? to) eqn:Hnz' in Hnz;
-          try (destruct signed in *; simpl in Hnz;
-               rewrite ?word.unsigned_of_Z_0, ?word.unsigned_of_Z_1 in Hnz;
-               congruence).
+          eexists; split. eauto using getmany0.
+          eexists; split. eauto using getmany1.
+          destruct signed; simpl;
+            rewrite ?lts_of_Z, ?ltu_of_Z by lia;
+            reflexivity. }
+        all:
+          pose proof Zlt_cases from' to;
+          intros Hnz; destruct (from' <? to);
+            try (rewrite ?word.unsigned_of_Z_0, ?word.unsigned_of_Z_1 in Hnz;
+                 congruence).
 
-        { (* Loop body analysis *)
-          apply Z.ltb_lt in Hnz'.
-          eapply compile_seq.
+        { eapply WeakestPrecondition_weaken; cycle 1.
           { (* User-supplied loop body *)
             unshelve apply Hbody; cycle -2.
             { unshelve apply Hcontinue; eassumption. }
             { apply Hpred. }
             all: eauto with arith || lia. }
-          { (* Variable increment *)
+          { (* Invariant proof *)
+            subst lp; cbv beta.
             set (body _ _ _ _) as acc_tok in *.
-            set (ExitToken.branch (fst acc_tok) (to - 1) from' + 1) as from'' in *.
+            set (ExitToken.branch (fst acc_tok) to (from' + 1)) as from'' in *.
 
-            subst lp; cbv beta; intros * (Hfromeq & Hlp).
-            eexists; split.
-            eexists; split; [exact Hfromeq|].
-            eexists; red. red.
-            simpl. rewrite <- word.ring_morph_add.
-            eexists; split; unfold inv.
+            intros * Hlp.
+            exists (Z.to_nat (to - from'')); split.
 
             assert (exists h,
                        acc_tok =
@@ -732,7 +784,7 @@ Section with_parameters.
               as [? Hrefold].
             { exists (ltac:(lia): from' + 1 <= to).
               subst acc_tok.
-              erewrite ranged_for'_unfold_r_nstop with (H := ?[H]).
+              erewrite ranged_for'_unfold_r_nstop with (H0 := ?[H]).
               [H]: lia.
               f_equal; f_equal; apply range_unique.
               cbv beta; intros; f_equal; apply range_unique.
@@ -740,7 +792,7 @@ Section with_parameters.
                 intros; cbv beta; f_equal; (congruence || lia || apply range_unique). }
 
             { (* Invariant proof *)
-              eexists from''.
+              exists from''.
 
               unshelve eexists;
                 [subst from''; destruct (fst acc_tok); simpl; lia|].
@@ -760,13 +812,11 @@ Section with_parameters.
                   intros; cbv beta; f_equal; (congruence || lia || apply range_unique). }
 
               { (* Final invariant holds *)
-                set (map.put _ from_var _) as locals' in *.
                 subst from'';
                   destruct (fst acc_tok) eqn:Htok; simpl in *;
                     rewrite Hrefold in Hlp.
                 { (* Loop exited early *)
                   erewrite ranged_for'_monotonic.
-                  replace (to - 1 + 1) with to in * by lia.
                   - eassumption.
                   - lia.
                   - cbv beta; intros; f_equal; apply range_unique.
@@ -780,7 +830,6 @@ Section with_parameters.
               subst from''. destruct (fst acc_tok); simpl; lia. } } }
 
         { (* Loop end analysis *)
-          apply Z.ltb_ge in Hnz'.
           cbv zeta in Hpred.
           assert (from' = to) as Hend by lia; destruct Hend.
           eapply Hk.
@@ -791,6 +840,97 @@ Section with_parameters.
             intros; cbv beta; f_equal; (congruence || lia || apply range_unique). } }
     Qed.
 
+    (* TODO Use a section? *)
+
+    Lemma compile_ranged_for_with_auto_increment A {tr mem locals functions}
+          (from to: Z) body (a0: A) :
+      let v := ranged_for from to body a0 in
+      forall {P} {pred: P v -> predicate}
+        (loop_pred: forall (idx: Z) (a: A), predicate)
+        {k: nlet_eq_k P v} {k_impl} {body_impl}
+        (from_var to_var: string) vars,
+
+        let lp from tok_acc tr mem locals :=
+            let from := ExitToken.branch (fst tok_acc) (to - 1) from in
+            loop_pred from (snd tok_acc) tr mem locals in
+
+        (forall from a0 tr mem locals,
+            loop_pred from a0 tr mem locals ->
+            map.getmany_of_list locals [from_var; to_var] =
+            Some [word.of_Z from; word.of_Z to]) ->
+
+        (forall from from' acc tr mem locals,
+            loop_pred from acc tr mem locals ->
+            loop_pred from' acc tr mem (map.put locals from_var (word.of_Z from'))) ->
+
+        loop_pred from a0 tr mem locals ->
+
+        (if signed then in_signed_bounds from /\ in_signed_bounds to
+         else in_unsigned_bounds from /\ in_unsigned_bounds to) ->
+
+        ((* loop body *)
+          let lp := lp in
+          forall tr mem locals from'
+            (Hl: from - 1 < from')
+            (Hr: from' < to)
+            (Hr': from' <= to),
+            let a := ranged_for' from from' (wbody body pr Hr') a0 in
+            let prev_tok := fst a in
+            let acc := snd a in  (* FIXME use primitive projections? *)
+            ExitToken.get prev_tok = false ->
+            loop_pred from' acc tr mem locals ->
+            (<{ Trace := tr;
+                Memory := mem;
+                Locals := locals;
+                Functions := functions }>
+             body_impl
+             <{ lp from' (body ExitToken.new from' acc (conj Hl Hr)) }>)) ->
+        (let v := v in
+         forall from' tr mem locals,
+           loop_pred from' v tr mem locals ->
+           (<{ Trace := tr;
+               Memory := mem;
+               Locals := locals;
+               Functions := functions }>
+            k_impl
+            <{ pred (k v eq_refl) }>)) ->
+        <{ Trace := tr;
+           Memory := mem;
+           Locals := locals;
+           Functions := functions }>
+        cmd.seq
+          (cmd.while
+             (expr.op (if signed then bopname.lts else bopname.ltu)
+                      (expr.var from_var)
+                      (expr.var to_var))
+             (cmd.seq body_impl
+                      (cmd.set from_var
+                               (expr.op bopname.add
+                                        (expr.var from_var)
+                                        (expr.literal 1)))))
+          k_impl
+        <{ pred (nlet_eq vars v k) }>.
+    Proof.
+      intros; eapply _compile_ranged_for; try eassumption.
+      (* Goal: (body; from := from + 1) does the right thing *)
+      intros; eapply compile_seq; eauto.
+      (* Goal: (from := from + 1) does the right thing *)
+
+      subst lp acc a; cbv beta; intros * Hlp.
+
+      eexists; split.
+      eexists; split.
+      eauto using getmany0.
+
+      simpl. red. red. rewrite <- word.ring_morph_add.
+      rewrite (ExitToken.map_branch (fun z => word.of_Z (z + 1))).
+      ring_simplify (to - 1 + 1).
+      rewrite <- ExitToken.map_branch.
+      reflexivity.
+
+      red. red. eauto.
+    Qed.
+
     Context {to_Z: word -> Z}
             (of_Z_to_Z: forall w, word.of_Z (to_Z w) = w)
             (to_Z_of_Z: forall l h w,
@@ -799,10 +939,8 @@ Section with_parameters.
 
     Lemma compile_ranged_for_w A {tr mem locals functions}
           (from to: word)
-          (H: if signed then
-                - 2 ^ (Semantics.width - 1) <=  to_Z from /\ to_Z to < 2 ^ (Semantics.width - 1)
-              else
-                0 <= to_Z from /\ to_Z to < 2 ^ Semantics.width)
+          (H: if signed then in_signed_bounds (to_Z from) /\ in_signed_bounds (to_Z to)
+              else in_unsigned_bounds (to_Z from) /\ in_unsigned_bounds (to_Z to))
           body (a0: A) :
       let v := ranged_for_w from to to_Z_of_Z body a0 in
       forall {P} {pred: P v -> predicate}
@@ -811,18 +949,19 @@ Section with_parameters.
         (from_var to_var: string) vars,
 
         let lp from tok_acc tr mem locals :=
-            let frm := ExitToken.branch (fst tok_acc) (word.sub to (word.of_Z 1)) from in
-            map.get locals from_var = Some frm /\
-            loop_pred (word.add frm (word.of_Z 1)) (snd tok_acc) tr mem
-                      (map.put locals from_var (word.add frm (word.of_Z 1))) in
+            let from := ExitToken.branch (fst tok_acc) (word.sub to (word.of_Z 1)) from in
+            loop_pred from (snd tok_acc) tr mem locals in
 
         (forall from a0 tr mem locals,
             loop_pred from a0 tr mem locals ->
             map.getmany_of_list locals [from_var; to_var] =
             Some [from; to]) ->
 
+        (forall from from' acc tr mem locals,
+            loop_pred from acc tr mem locals ->
+            loop_pred from' acc tr mem (map.put locals from_var from')) ->
+
         loop_pred from a0 tr mem locals ->
-        to_Z from <= to_Z to ->
 
         ((* loop body *)
           let lp := lp in
@@ -830,7 +969,7 @@ Section with_parameters.
             (Hl: to_Z from - 1 < to_Z from')
             (Hr: to_Z from' < to_Z to)
             (Hr': to_Z from' <= to_Z to),
-            let tok := ExitToken.new false in
+            let tok := ExitToken.new in
             let a := ranged_for' (to_Z from) (to_Z from')
                                 (w_body _ _ to_Z_of_Z
                                         (wbody body pr Hr')) a0 in
@@ -844,8 +983,8 @@ Section with_parameters.
              body_impl
              <{ lp from' (body tok from' (snd a) (conj Hl Hr)) }>)) ->
         (let v := v in
-         forall tr mem locals,
-           loop_pred to v tr mem locals ->
+         forall from' tr mem locals,
+           loop_pred from' v tr mem locals ->
            (<{ Trace := tr;
                Memory := mem;
                Locals := locals;
@@ -870,15 +1009,16 @@ Section with_parameters.
           k_impl
         <{ pred (nlet_eq vars v k) }>.
     Proof.
-      intros * Hlocals Hinit Hfromto Hbody Hk.
-      apply compile_ranged_for
-        with (loop_pred := fun z => loop_pred (word.of_Z z)); intros.
+      intros * Hlocals Hfromindep Hinit Hbody Hk.
+      apply compile_ranged_for_with_auto_increment
+        with (loop_pred := fun z => loop_pred (word.of_Z z)).
 
-      - rewrite of_Z_to_Z. eauto.
+      - rewrite of_Z_to_Z; eauto.
+      - eauto.
       - rewrite of_Z_to_Z; eassumption.
       - eassumption.
-      - eassumption.
-      - assert (exists h, a = ranged_for' (to_Z from) (to_Z (word.of_Z from')) (w_body from (word.of_Z from') to_Z_of_Z (wbody body pr h)) a0) as [h eqn].
+      - intros.
+        assert (exists h, a = ranged_for' (to_Z from) (to_Z (word.of_Z from')) (w_body from (word.of_Z from') to_Z_of_Z (wbody body pr h)) a0) as [h eqn].
         { unshelve eexists; subst a.
           { rewrite (to_Z_of_Z from to); lia. }
           unshelve apply ranged_for'_Proper; reflexivity || eauto.
@@ -897,12 +1037,11 @@ Section with_parameters.
           { subst b0 b1. f_equal. apply range_unique. }
           clearbody b0; subst.
 
-          intros * (Hm & Hlp).
+          intros * Hlp.
           * destruct (fst b1); simpl in *;
               repeat rewrite ?word.ring_morph_add, ?word.ring_morph_sub, ?of_Z_to_Z;
               eauto.
-      - eapply Hk.
-        rewrite of_Z_to_Z in H0.
+      - intros; eapply Hk.
         eassumption.
     Qed.
   End Generic.
@@ -914,31 +1053,15 @@ Section with_parameters.
           {functions : list (string * (list string * list string * cmd))}
           (from to : word).
 
-  Let unsigned_bounds:
-    0 <= word.unsigned from /\
-    word.unsigned to < 2 ^ Semantics.width.
-  Proof.
-    pose proof word.unsigned_range from;
-      pose proof word.unsigned_range to.
-    lia.
-  Qed.
-
-  Let signed_bounds:
-    - 2 ^ (Semantics.width - 1) <= word.signed from /\
-    word.signed to < 2 ^ (Semantics.width - 1).
-  Proof.
-    pose proof word.signed_range from;
-      pose proof word.signed_range to.
-    lia.
-  Qed.
-
   Definition compile_ranged_for_u :=
     @compile_ranged_for_w false _ word.of_Z_unsigned word_unsigned_of_Z_bracketed
-                          A tr mem locals functions from to unsigned_bounds.
+                          A tr mem locals functions from to
+                          (conj (word.unsigned_range _) (word.unsigned_range _)).
 
   Definition compile_ranged_for_s :=
     @compile_ranged_for_w true _ word.of_Z_signed word_signed_of_Z_bracketed
-                          A tr mem locals functions from to signed_bounds.
+                          A tr mem locals functions from to
+                          (conj (word.signed_range _) (word.signed_range _)).
 End with_parameters.
 
 Require bedrock2.BasicC64Semantics.
@@ -949,7 +1072,7 @@ Module test.
   Time Compute (ranged_for 0 15
                         (fun t idx acc _ =>
                            if Z.ltb 11 idx then
-                             let t' := ExitToken.set t in
+                             let t' := ExitToken.break t in
                              (t', acc)
                            else
                              let acc := idx :: acc in
@@ -958,7 +1081,7 @@ Module test.
   Time Compute (ranged_for_u (word.of_Z 0) (word.of_Z 15)
                           (fun t idx acc _ =>
                              if word.ltu (word.of_Z 11) idx then
-                               let t' := ExitToken.set t in
+                               let t' := ExitToken.break t in
                                (t', acc)
                              else
                                let acc := idx :: acc in
